Removed unnecessary assertions

iso-dh/ISODH.SecurityLemmas.fst
@@ -9,13 +9,9 @@ let responder_correspondence_lemma i a b gx gy k = ()
 let key_secrecy_lemma k a b = secrecy_join_label_lemma #(pki isodh) k 
 
 let initiator_forward_secrecy_lemma i a b gx gy k =
-  let t0 = global_timestamp () in
-  assert (later_than t0 i);
   key_secrecy_lemma k a b;
   ()
   
 let responder_forward_secrecy_lemma i a b gx gy k =
-  let t0 = global_timestamp () in
-  assert (later_than t0 i);
   key_secrecy_lemma k a b;
   ()
