iso-dh/ISODH.SecurityLemmas.fsti
@@ -33,14 +33,14 @@ val key_secrecy_lemma : k:bytes -> a:principal -> b:principal ->
 
 val initiator_forward_secrecy_lemma: i:nat -> a:principal -> b:principal -> gx:bytes -> gy:bytes -> k:bytes -> 
     LCrypto unit (pki isodh)
-    (requires (fun t0 -> i < trace_len t0 /\ did_event_occur_at i a (finishI a b gx gy k)))
+    (requires (fun t0 -> (later_than (trace_len t0) i /\ (i <> trace_len t0)) /\ did_event_occur_at i a (finishI a b gx gy k)))
     (ensures (fun t0 _ t1 -> t0 == t1 /\ (corrupt_at i (P b) \/ 
 	     (exists si sj vi vj. is_labeled isodh_global_usage i k (join (readers [V a si vi]) (readers [V b sj vj])) /\ 
 			     (corrupt_at (trace_len t0) (V a si vi) \/ corrupt_at (trace_len t0) (V b sj vj) \/ is_unknown_to_attacker_at (trace_len t0) k)))))
 
 val responder_forward_secrecy_lemma: i:nat -> a:principal -> b:principal -> gx:bytes -> gy:bytes -> k:bytes ->  
     LCrypto unit (pki isodh)
-    (requires (fun t0 -> i < trace_len t0 /\ did_event_occur_at i b (finishR a b gx gy k)))
+    (requires (fun t0 -> (later_than (trace_len t0) i /\ (i <> trace_len t0)) /\ did_event_occur_at i b (finishR a b gx gy k)))
     (ensures (fun t0 _ t1 -> t0 == t1 /\ (corrupt_at i (P a) \/ 
 	     (exists si sj vi vj. is_labeled isodh_global_usage i k (join (readers [V b si vi]) (readers [V a sj vj])) /\ 
 			     (corrupt_at (trace_len t0) (V b si vi) \/ corrupt_at (trace_len t0) (V a sj vj) \/ is_unknown_to_attacker_at (trace_len t0) k)))))
